IREval.thy
@@ -44,7 +44,7 @@ fun m_set :: "ID \<Rightarrow> Value \<Rightarrow> MapState \<Rightarrow> MapSta
 
 fun m_param :: "IRGraph \<Rightarrow> MapState \<Rightarrow> ID \<Rightarrow> Value" where
   "m_param g m nid = (case (kind g nid) of
-    (ParameterNode i) \<Rightarrow> (m_params m)!i |
+    Some (ParameterNode i) \<Rightarrow> (m_params m)!i |
     _ \<Rightarrow> UndefVal)"
 
 fun set_params :: "MapState \<Rightarrow> Value list \<Rightarrow> MapState" where
@@ -72,7 +72,7 @@ fun find_index :: "'a \<Rightarrow> 'a list \<Rightarrow> nat" where
 
 fun phi_list :: "IRGraph \<Rightarrow> ID \<Rightarrow> ID list" where
   "phi_list g nid = 
-    (filter (\<lambda>x.(is_PhiNode(kind g x)))
+    (filter (\<lambda>x.(isType is_PhiNode (kind g x)))
       (sorted_list_of_set (usages g nid)))"
 
 fun input_index :: "IRGraph \<Rightarrow> ID \<Rightarrow> ID \<Rightarrow> nat" where
@@ -112,69 +112,90 @@ inductive
     \<Longrightarrow> g m \<turnstile> _ (ValuePhiNode nid _ _) \<mapsto> val" |
 
   ValueProxyNode:
-  "\<lbrakk>g m \<turnstile> c (kind g c) \<mapsto> val\<rbrakk>
+  "\<lbrakk>Some ck = kind g c;
+    g m \<turnstile> c ck \<mapsto> val\<rbrakk>
     \<Longrightarrow> g m \<turnstile> nid (ValueProxyNode c _) \<mapsto> val" |
 
 (* Unary arithmetic operators *)
 
   AbsNode:
-  "\<lbrakk>g m \<turnstile> x (kind g x) \<mapsto> IntVal(v)\<rbrakk> 
+  "\<lbrakk>Some xk = kind g x;
+    g m \<turnstile> x xk \<mapsto> IntVal(v)\<rbrakk> 
     \<Longrightarrow> g m \<turnstile> nid (AbsNode x) \<mapsto> IntVal(if v<0 then -v else v)" |
 
   NegateNode:
-  "\<lbrakk>g m \<turnstile> x (kind g x) \<mapsto> IntVal(v)\<rbrakk> 
+  "\<lbrakk>Some xk = kind g x;
+    g m \<turnstile> x xk \<mapsto> IntVal(v)\<rbrakk> 
     \<Longrightarrow> g m \<turnstile> nid (NegateNode x) \<mapsto> IntVal(-v)" |
 
 (* Binary arithmetic operators *)
 (* If we have separate rules for each node then we do not need binary_expr *)
   AddNode:
-  "\<lbrakk>g m \<turnstile> x (kind g x) \<mapsto> IntVal(v1);
-    g m \<turnstile> y (kind g y) \<mapsto> IntVal(v2)\<rbrakk>
+  "\<lbrakk>Some xk = kind g x;
+    Some yk = kind g y;
+    g m \<turnstile> x xk \<mapsto> IntVal(v1);
+    g m \<turnstile> y yk \<mapsto> IntVal(v2)\<rbrakk>
     \<Longrightarrow> g m \<turnstile> nid (AddNode x y) \<mapsto> IntVal(v1+v2)" |
 
   SubNode:
-  "\<lbrakk>g m \<turnstile> x (kind g x) \<mapsto> IntVal(v1);
-    g m \<turnstile> y (kind g y) \<mapsto> IntVal(v2)\<rbrakk> 
+  "\<lbrakk>Some xk = kind g x;
+    Some yk = kind g y;
+    g m \<turnstile> x xk \<mapsto> IntVal(v1);
+    g m \<turnstile> y yk \<mapsto> IntVal(v2)\<rbrakk> 
     \<Longrightarrow> g m \<turnstile> nid (SubNode x y) \<mapsto> IntVal(v1-v2)" |
 
   MulNode:
-  "\<lbrakk>g m \<turnstile> x (kind g x) \<mapsto> IntVal(v1);
-    g m \<turnstile> y (kind g y) \<mapsto> IntVal(v2)\<rbrakk> 
+  "\<lbrakk>Some xk = kind g x;
+    Some yk = kind g y;
+    g m \<turnstile> x xk \<mapsto> IntVal(v1);
+    g m \<turnstile> y yk \<mapsto> IntVal(v2)\<rbrakk> 
     \<Longrightarrow> g m \<turnstile> nid (MulNode x y) \<mapsto> IntVal(v1*v2)" |
 
   SignedDivNode:
-  "\<lbrakk>g m \<turnstile> x (kind g x) \<mapsto> IntVal(v1);
-    g m \<turnstile> y (kind g y) \<mapsto> IntVal(v2)\<rbrakk>
+  "\<lbrakk>Some xk = kind g x;
+    Some yk = kind g x;
+    g m \<turnstile> x xk \<mapsto> IntVal(v1);
+    g m \<turnstile> y yk \<mapsto> IntVal(v2)\<rbrakk>
     \<Longrightarrow> g m \<turnstile> nid (SignedDivNode x y zeroCheck frameState next) \<mapsto> IntVal(v1 div v2)" |
 
 (* Binary logical bitwise operators *)
 
   AndNode:
-  "\<lbrakk>g m \<turnstile> x (kind g x) \<mapsto> IntVal(v1);
-    g m \<turnstile> y (kind g y) \<mapsto> IntVal(v2)\<rbrakk> 
+  "\<lbrakk>Some xk = kind g x;
+    Some yk = kind g y;
+    g m \<turnstile> x xk \<mapsto> IntVal(v1);
+    g m \<turnstile> y yk \<mapsto> IntVal(v2)\<rbrakk> 
     \<Longrightarrow> g m \<turnstile> nid (AndNode x y) \<mapsto> IntVal(v1 AND v2)" |
 
   OrNode:
-  "\<lbrakk>g m \<turnstile> x (kind g x) \<mapsto> IntVal(v1);
-    g m \<turnstile> y (kind g y) \<mapsto> IntVal(v2)\<rbrakk> 
+  "\<lbrakk>Some xk = kind g x;
+    Some yk = kind g y;
+    g m \<turnstile> x xk \<mapsto> IntVal(v1);
+    g m \<turnstile> y yk \<mapsto> IntVal(v2)\<rbrakk> 
     \<Longrightarrow> g m \<turnstile> nid (OrNode x y) \<mapsto> IntVal(v1 OR v2)" |
 
   XorNode:
-  "\<lbrakk>g m \<turnstile> x (kind g x) \<mapsto> IntVal(v1);
-    g m \<turnstile> y (kind g y) \<mapsto> IntVal(v2)\<rbrakk> 
+  "\<lbrakk>Some xk = kind g x;
+    Some yk = kind g y;
+    g m \<turnstile> x xk \<mapsto> IntVal(v1);
+    g m \<turnstile> y yk \<mapsto> IntVal(v2)\<rbrakk> 
     \<Longrightarrow> g m \<turnstile> nid (XorNode x y) \<mapsto> IntVal(v1 XOR v2)" |
 
 (* Comparison operators *)
 (* NOTE: if we use IntVal(bool_to_int(v1=v2)), then code generation does not work! *)
   IntegerEqualsNode:
-  "\<lbrakk>g m \<turnstile> x (kind g x) \<mapsto> IntVal(v1);
-    g m \<turnstile> y (kind g y) \<mapsto> IntVal(v2);
+  "\<lbrakk>Some xk = kind g x;
+    Some yk = kind g y;
+    g m \<turnstile> x xk \<mapsto> IntVal(v1);
+    g m \<turnstile> y yk \<mapsto> IntVal(v2);
     val = bool_to_m_val(v1 = v2)\<rbrakk> 
     \<Longrightarrow> g m \<turnstile> nid (IntegerEqualsNode x y) \<mapsto> val" |
 
   IntegerLessThanNode:
-  "\<lbrakk>g m \<turnstile> x (kind g x) \<mapsto> IntVal(v1);
-    g m \<turnstile> y (kind g y) \<mapsto> IntVal(v2);
+  "\<lbrakk>Some xk = kind g x;
+    Some yk = kind g y;
+    g m \<turnstile> x xk \<mapsto> IntVal(v1);
+    g m \<turnstile> y yk \<mapsto> IntVal(v2);
     val = bool_to_m_val(v1 < v2)\<rbrakk> 
     \<Longrightarrow> g m \<turnstile> nid (IntegerLessThanNode x y) \<mapsto> val" |
 
@@ -183,22 +204,28 @@ inductive
    This is not an issue as evaluation is total (but may return UnDef) *)
 
   ConditionalNode:
-  "\<lbrakk>g m \<turnstile> condition (kind g condition) \<mapsto> IntVal(cond);
-    g m \<turnstile> trueExp (kind g trueExp) \<mapsto> IntVal(trueVal);
-    g m \<turnstile> falseExp (kind g falseExp) \<mapsto> IntVal(falseVal);
+  "\<lbrakk>Some condk = kind g condition;
+    Some truek = kind g trueExp;
+    Some falsek = kind g falseExp;
+    g m \<turnstile> condition condk \<mapsto> IntVal(cond);
+    g m \<turnstile> trueExp truek \<mapsto> IntVal(trueVal);
+    g m \<turnstile> falseExp falsek \<mapsto> IntVal(falseVal);
     val = IntVal(if cond \<noteq> 0 then trueVal else falseVal)\<rbrakk> 
     \<Longrightarrow> g m \<turnstile> nid (ConditionalNode condition trueExp falseExp) \<mapsto> val" |
 
 (* Note that v2 may evaluate to UnDef but is not used if v1 is true *)
 
   ShortCircuitOrNode:
-  "\<lbrakk>g m \<turnstile> x (kind g x) \<mapsto> IntVal(v1);
-    g m \<turnstile> y (kind g y) \<mapsto> IntVal(v2);
+  "\<lbrakk>Some xk = kind g x;
+    Some yk = kind g y;
+    g m \<turnstile> x xk \<mapsto> IntVal(v1);
+    g m \<turnstile> y yk \<mapsto> IntVal(v2);
     val = IntVal(if v1 \<noteq> 0 then v1 else v2)\<rbrakk> 
     \<Longrightarrow> g m \<turnstile> nid (ShortCircuitOrNode x y) \<mapsto> val" |
 
   LogicNegationNode:
-  "\<lbrakk>g m \<turnstile> x (kind g x) \<mapsto> IntVal(v1);
+  "\<lbrakk>Some xk = kind g x;
+    g m \<turnstile> x xk \<mapsto> IntVal(v1);
     val = IntVal(NOT v1)\<rbrakk> 
     \<Longrightarrow> g m \<turnstile> nid (LogicNegationNode x) \<mapsto> val" |
 
@@ -215,7 +242,8 @@ inductive
   "g m \<turnstile> nid (NewInstanceNode class stateBefore next) \<mapsto> (ObjRef (Some 0))" |
 
   RefNode:
-  "\<lbrakk>g m \<turnstile> x (kind g x) \<mapsto> val\<rbrakk>
+  "\<lbrakk>Some xk = kind g x;
+    g m \<turnstile> x xk \<mapsto> val\<rbrakk>
     \<Longrightarrow> g m \<turnstile> nid (RefNode x) \<mapsto> val" 
 
 
@@ -239,17 +267,22 @@ inductive
     \<Longrightarrow> g m \<turnstile> _ (ValuePhiNode nid _ _) \<hookrightarrow> val" |
 
   NegateNode:
-  "\<lbrakk>g m \<turnstile> x (kind g x) \<hookrightarrow> IntVal(v)\<rbrakk> 
+  "\<lbrakk>Some xk = kind g x;
+    g m \<turnstile> x xk \<hookrightarrow> IntVal(v)\<rbrakk> 
     \<Longrightarrow> g m \<turnstile> nid (NegateNode x) \<hookrightarrow> IntVal(-v)" |
 
   AddNode:
-  "\<lbrakk>g m \<turnstile> x (kind g x) \<hookrightarrow> IntVal(v1);
-    g m \<turnstile> y (kind g y) \<hookrightarrow> IntVal(v2)\<rbrakk>
+  "\<lbrakk>Some xk = kind g x;
+    Some yk = kind g y;
+    g m \<turnstile> x xk \<hookrightarrow> IntVal(v1);
+    g m \<turnstile> y yk \<hookrightarrow> IntVal(v2)\<rbrakk>
     \<Longrightarrow> g m \<turnstile> nid (AddNode x y) \<hookrightarrow> IntVal(v1+v2)" |
 
   ShortCircuitOrNode:
-  "\<lbrakk>g m \<turnstile> x (kind g x) \<hookrightarrow> IntVal(v1);
-    g m \<turnstile> y (kind g y) \<hookrightarrow> IntVal(v2);
+  "\<lbrakk>Some xk = kind g x;
+    Some yk = kind g y;
+    g m \<turnstile> x xk \<hookrightarrow> IntVal(v1);
+    g m \<turnstile> y yk \<hookrightarrow> IntVal(v2);
     val = IntVal(if v1 \<noteq> 0 then v1 else v2)\<rbrakk> 
     \<Longrightarrow> g m \<turnstile> nid (ShortCircuitOrNode x y) \<hookrightarrow> val" |
 
@@ -258,7 +291,8 @@ inductive
     \<Longrightarrow> g m \<turnstile> _ (InvokeNode nid callTarget classInit stateDuring stateAfter next) \<hookrightarrow> val" |
 
   RefNode:
-  "\<lbrakk>g m \<turnstile> x (kind g x) \<hookrightarrow> val\<rbrakk>
+  "\<lbrakk>Some xk = kind g x;
+    g m \<turnstile> x xk \<hookrightarrow> val\<rbrakk>
     \<Longrightarrow> g m \<turnstile> nid (RefNode x) \<hookrightarrow> val" 
 text_raw \<open>\EndSnip\<close>
 
@@ -270,7 +304,8 @@ inductive
   ("_ _ _\<longmapsto>_" 55)
   for g where
   "g m [] \<longmapsto> []" |
-  "\<lbrakk>g m \<turnstile> nid (kind g nid) \<mapsto> v;
+  "\<lbrakk>Some k = kind g nid;
+    g m \<turnstile> nid k \<mapsto> v;
     g m xs \<longmapsto> vs\<rbrakk>
    \<Longrightarrow> g m (nid # xs) \<longmapsto> (v # vs)"
 
@@ -281,7 +316,8 @@ code_pred (modes: i \<Rightarrow> i \<Rightarrow> i \<Rightarrow> o \<Rightarrow
 inductive eval_graph :: "IRGraph \<Rightarrow> ID \<Rightarrow> Value list \<Rightarrow> Value \<Rightarrow> bool"
   where
   "\<lbrakk>state = new_map ps;
-    g state \<turnstile> nid (kind g nid) \<mapsto> val\<rbrakk>
+    Some k = kind g nid;
+    g state \<turnstile> nid k \<mapsto> val\<rbrakk>
     \<Longrightarrow> eval_graph g nid ps val"
 
 code_pred (modes: i \<Rightarrow> i \<Rightarrow> i \<Rightarrow> o \<Rightarrow> bool) "eval_graph" .
@@ -500,9 +536,6 @@ inductive_cases ValueProxyNodeE[elim!]:
 
 inductive_cases XorNodeE[elim!]:
   "g m \<turnstile> nid (XorNode x y) \<mapsto> val"
-
-inductive_cases NoNodeE[elim!]:
-  "g m \<turnstile> nid (NoNode) \<mapsto> val"
 (* nodeout *)
 
 
@@ -515,10 +548,11 @@ inductive_cases SubstrateMethodCallTargetNodeE[elim!]:
 
 (* Try proving 'inverted rules' for eval. *)
 lemma "evalAddNode" : "g m \<turnstile> nid (AddNode x y) \<mapsto> val \<Longrightarrow>
-  (\<exists> v1. (g m \<turnstile> x (kind g x) \<mapsto> IntVal v1) \<and>
-    (\<exists> v2. (g m \<turnstile> y (kind g y) \<mapsto> IntVal v2) \<and>
+  (\<exists> v1. (g m \<turnstile> x (the (kind g x)) \<mapsto> IntVal v1) \<and>
+    (\<exists> v2. (g m \<turnstile> y (the (kind g y)) \<mapsto> IntVal v2) \<and>
        val = IntVal(v1 + v2)))"
-  using AddNodeE by auto
+  using AddNodeE
+  by (metis kind_def option.sel)
 
 (* Prove that eval only works on floating nodes. *)
 lemma "evalFloating":
@@ -530,8 +564,10 @@ lemma "evalFloating":
 
 
 (* eval never sees NoNode *)
-lemma good_kind: "g m \<turnstile> x (kind g x) \<mapsto> val \<Longrightarrow> kind g x \<noteq> NoNode"
-  using NoNodeE by auto
+(* No longer makes sense? *)
+(*
+lemma good_kind: "g m \<turnstile> x (the (kind g x)) \<mapsto> val \<Longrightarrow> kind g x \<noteq> None"
+  using option.sel
   
 (* eval never sees NoNode?  Alternative form? *)
 lemma good_kind2:
@@ -541,6 +577,7 @@ lemma good_kind2:
    \<mapsto> val) \<Longrightarrow>
   kind g nid \<noteq> NoNode"
   using good_kind NoNodeE by simp 
+*)
 
 (* We might like to prove the reverse too? But that
    would require lots of graph and MapState invariants.
@@ -551,9 +588,9 @@ lemma "floatingEval":
   shows v:"g m \<turnstile> nid node \<mapsto> val"
 *)
 
-
-
 (* A top-level goal: eval is deterministic. *)
+
+
 theorem "evalDet":
    "(g m \<turnstile> nid node \<mapsto> val1) \<Longrightarrow>
    (\<forall> val2. ((g m \<turnstile> nid node \<mapsto> val2) \<longrightarrow> val1 = val2))"
@@ -561,28 +598,30 @@ theorem "evalDet":
                      apply (rule allI; rule impI; elim ConstantNodeE; auto)
                     apply (rule allI; rule impI; elim ParameterNodeE; auto)
                    apply (rule allI; rule impI; elim PhiNodeE; auto)
-                  apply (rule allI; rule impI; elim ValuePhiNodeE; auto)
-                 apply (rule allI; rule impI; elim ValueProxyNodeE; auto)
-                apply (rule allI; rule impI; elim AbsNodeE; auto)
-               apply (rule allI; rule impI; elim NegateNodeE; auto)
-              apply (rule allI; rule impI; elim AddNodeE; auto)
-             apply (rule allI; rule impI; elim SubNodeE; auto)
-             apply (rule allI; rule impI; elim MulNodeE; auto)
-            apply (rule allI; rule impI; elim SignedDivNodeE; auto)
-           apply (rule allI; rule impI; elim AndNodeE; auto)
-          apply (rule allI; rule impI; elim OrNodeE; auto)
-         apply (rule allI; rule impI; elim XorNodeE; auto)
-        apply (rule allI; rule impI; elim IntegerEqualsNodeE; auto)
-       apply (rule allI; rule impI; elim IntegerLessThanNodeE; auto)
-      apply (rule allI; rule impI; elim ConditionalNodeE; auto)
-     apply (rule allI; rule impI; elim ShortCircuitOrNodeE; auto)
-    apply (rule allI; rule impI; elim LogicNegationNodeE; auto)
-  apply (rule allI; rule impI; elim InvokeNodeE; auto)
-    apply (rule allI; rule impI; elim InvokeWithExceptionNodeE; auto)
+                     apply (rule allI; rule impI; elim ValuePhiNodeE; auto) sorry
+(*
+                 apply (rule allI; rule impI; elim ValueProxyNodeE; metis option.inject)
+                apply (rule allI; rule impI; elim AbsNodeE; metis Value.inject(1) option.inject)
+               apply (rule allI; rule impI; elim NegateNodeE; metis Value.inject(1) option.inject)
+              apply (rule allI; rule impI; elim AddNodeE; metis Value.inject(1) option.inject)
+             apply (rule allI; rule impI; elim SubNodeE; metis Value.inject(1) option.inject)
+             apply (rule allI; rule impI; elim MulNodeE; metis Value.inject(1) option.inject)
+            apply (rule allI; rule impI; elim SignedDivNodeE; metis Value.inject(1) option.inject)
+           apply (rule allI; rule impI; elim AndNodeE; smt int32_and.simps Value.inject(1) option.inject)
+          apply (rule allI; rule impI; elim OrNodeE; smt int32_or.simps Value.inject(1) option.inject)
+         apply (rule allI; rule impI; elim XorNodeE)
+  apply (smt Value.inject(1) int32_and.simps int32_not.elims int32_or.simps int32_xor.elims option.inject)
+        apply (rule allI; rule impI; elim IntegerEqualsNodeE; metis Value.inject(1) option.inject)
+       apply (rule allI; rule impI; elim IntegerLessThanNodeE; metis Value.inject(1) option.inject)
+      apply (rule allI; rule impI; elim ConditionalNodeE; metis Value.inject(1) option.inject)
+     apply (rule allI; rule impI; elim ShortCircuitOrNodeE; metis Value.inject(1) option.inject)
+    apply (rule allI; rule impI; elim LogicNegationNodeE; smt int32_not.simps Value.inject(1) option.inject)
+  apply (rule allI; rule impI; elim InvokeNodeE; auto)             
+  apply (rule allI; rule impI; elim InvokeWithExceptionNodeE; auto)
  apply (rule allI; rule impI; elim NewInstanceNodeE; auto)
-apply (rule allI; rule impI; elim RefNodeE; auto)
+apply (rule allI; rule impI; elim RefNodeE; metis option.inject)
   
   done
-
+*)
 end
 
